uniqueHeap/unspec.v
@@ -9,14 +9,24 @@ Require Import classifiedStep.
 Require Import hetList. 
 Require Import Coq.Sets.Ensembles. 
 
+Definition commit a :=
+  match a with
+      |unlocked nil => true
+      |_ => false
+  end. 
+
 (*------------------------------------Unspec Definitions----------------------------*)
 Fixpoint raw_unspecHeap (H : rawHeap ivar_state) :=
   match H with
-      |(i, sempty (hd::tl))::H' => raw_unspecHeap H'
-      |(i, sempty nil)::H' => (i, sempty nil)::raw_unspecHeap H'
-      |(i, sfull (hd::tl) _ _ _ _)::H' => raw_unspecHeap H'
-      |(i, sfull nil _ (hd::tl) _ _) :: H' => (i, sempty nil)::raw_unspecHeap H'
-      |(i, sfull nil ds nil t M)::H' => (i, sfull nil (Empty_set tid) nil t M)::raw_unspecHeap H'
+      |(i, sempty a)::H' => if commit a 
+                            then (i, sempty a)::raw_unspecHeap H'
+                            else raw_unspecHeap H'
+      |(i, sfull a1 a2 a3 a4 a5) :: H' =>
+       if commit a1
+       then if commit a3
+            then (i, sfull a1 (Empty_set tid) a3 a4 a5)::raw_unspecHeap H'
+            else (i, sempty a1) :: raw_unspecHeap H'
+       else raw_unspecHeap H'
       |nil => nil
   end. 
 
@@ -26,22 +36,16 @@ Theorem unspecMonotonic : forall h u,
                             monotonic u ivar_state h ->
                             monotonic u ivar_state (raw_unspecHeap h). 
 Proof.
-  induction h; intros; auto. destruct a. 
+  induction h; intros; auto. simpl in *. destruct a. 
   {destruct i0; auto. 
-   {destruct a. simpl. inv H. constructor. auto. eauto. simpl. inv H. 
+   {destruct (commit a). simpl. inv H. constructor. auto. eauto. simpl. inv H. 
     eapply monotonicLowerUB; eauto. }
-   {destruct a. 
-    {simpl. destruct a0. 
-     {inv H. constructor; auto. }
-     {inv H. constructor; auto. }
-    }
-    {destruct a0. 
-     {simpl. inv H. eapply monotonicLowerUB; eauto. }
-     {simpl. inv H. eapply monotonicLowerUB; eauto. }
-    }
+   {destruct (commit a). 
+    {destruct (commit a0). inv H. eauto. inv H. eauto. }
+    {inv H. eapply monotonicLowerUB; eauto. }
    }
   }
-Qed. 
+Qed.  
 
 Definition unspecHeap H := 
   match H with
@@ -50,24 +54,24 @@ Definition unspecHeap H :=
 
 Inductive unspecThread : thread -> Ensemble thread -> Prop :=
 |unspecCommit : forall tid s2 M,
-                  unspecThread (tid, nil, s2, M) (tSingleton(tid, nil, s2, M))
+                  unspecThread (tid, unlocked nil, s2, M) (tSingleton(tid, unlocked nil, s2, M))
 |unspecRead : forall tid s1 s1' s2 M i t E (d:decompose t E (get (fvar i))),
-             s1 = s1' ++ [rAct i t E d] -> 
-             unspecThread (tid, s1, s2, M) (tSingleton(tid, nil, s2, t))
+             s1 = unlocked(s1' ++ [rAct i t E d]) -> 
+             unspecThread (tid, s1, s2, M) (tSingleton(tid, unlocked nil, s2, t))
 |unspecWrite : forall tid s1 s1' s2 M M' i c t (d:decompose t c (put (fvar i) M')),
-       s1 = s1' ++ [wAct i t c M' d] ->
-       unspecThread (tid, s1, s2, M) (tSingleton(tid, nil, s2, t))
+       s1 = unlocked(s1' ++ [wAct i t c M' d]) ->
+       unspecThread (tid, s1, s2, M) (tSingleton(tid, unlocked nil, s2, t))
 |unspecCreate : forall tid s1 s1' s2 M i c t (d:decompose t c new),
-                  s1 = s1' ++ [nAct t c d i] ->
-                  unspecThread (tid, s1, s2, M) (tSingleton(tid, nil, s2, t))
-|unSpecFork : forall c tid s1 s1' s2 M M' t (d:decompose t c (fork M')),
-                s1 = s1' ++ [fAct t c M' d] ->
-                unspecThread (tid, s1, s2, M) (tSingleton(tid, nil, s2, t))
-|unSpecSpecret : forall t c M M' N tid s1 s1' s2 (d:decompose t c (spec M' N)), 
-                   s1 = s1' ++ [srAct t c M' N d] ->
-                   unspecThread(tid, s1, s2, M) (tSingleton(tid, nil, s2, t))
-|unspecCreatedSpec : forall s1 s1' s2 M tid,
-                       s1 = s1' ++ [specAct] -> unspecThread (tid, s1, s2, M) tEmptySet
+                  s1 = unlocked(s1' ++ [nAct t c d i]) ->
+                  unspecThread (tid, s1, s2, M) (tSingleton(tid, unlocked nil, s2, t))
+|unspecFork : forall c tid s1 s1' s2 M M' t (d:decompose t c (fork M')),
+                s1 = unlocked(s1' ++ [fAct t c M' d]) ->
+                unspecThread (tid, s1, s2, M) (tSingleton(tid, unlocked nil, s2, t))
+|unspecSpecret : forall t c M M' N tid s1 s1' s2 (d:decompose t c (spec M' N)), 
+                   s1 = unlocked(s1' ++ [srAct t c M' N d]) ->
+                   unspecThread(tid, s1, s2, M) (tSingleton(tid, unlocked nil, s2, t))
+|unspecLocked : forall tid s1 s2 M, 
+                  unspecThread (tid, locked s1, s2, M) tEmptySet
 . 
 
 Hint Constructors unspecThread. 
@@ -86,7 +90,7 @@ Inductive wellFormed : sHeap -> pool -> Prop :=
                      wellFormed H T
 .
 
-Definition commitPool (T:pool) : Prop := forall tid s1 s2 M, tIn T (tid, s1, s2, M) -> s1 = nil. 
+Definition commitPool (T:pool) : Prop := forall tid s1 s2 M, tIn T (tid, s1, s2, M) -> s1 = unlocked nil. 
 
 Inductive actionTerm : action -> trm -> Prop :=
 |basicRead : forall x t E d, actionTerm (rAct x t E d) t
@@ -99,31 +103,30 @@ Hint Resolve app_comm_cons app_nil_l.
 
 Ltac unspecThreadTac :=
   match goal with
-    | |-unspecThread(?t, [], ?s, ?m) ?z => eapply unspecCommit
-    | |-unspecThread(?t, ?x++[rAct ?a ?b ?c ?d], ?s, ?m) ?z => eapply unspecRead
-    | |-unspecThread(?t, ?x++[wAct ?a ?b ?c ?d ?e], ?s, ?m) ?z => eapply unspecWrite
-    | |-unspecThread(?t, ?x++[nAct ?a ?b ?c ?d], ?s, ?m) ?z => eapply unspecCreate
-    | |-unspecThread(?t, ?x++[fAct ?a ?b ?c ?d], ?s, ?m) ?z => eapply unSpecFork
-    | |-unspecThread(?t, ?x++[srAct ?a ?b ?c ?d ?e], ?s, ?m) ?z => eapply unSpecSpecret
-    | |-unspecThread(?t, ?x++[specAct], ?s, ?m) ?z => eapply unspecCreatedSpec
-    | |-unspecThread(?t, [rAct ?a ?b ?c ?d], ?s, ?m) ?z => eapply unspecRead
-    | |-unspecThread(?t, [wAct ?a ?b ?c ?d ?e], ?s, ?m) ?z => eapply unspecWrite
-    | |-unspecThread(?t, [nAct ?a ?b ?c ?d], ?s, ?m) ?z => eapply unspecCreate
-    | |-unspecThread(?t, [fAct ?a ?b ?c ?d], ?s, ?m) ?z => eapply unSpecFork
-    | |-unspecThread(?t, [srAct ?a ?b ?c ?d ?e], ?s, ?m) ?z => eapply unSpecSpecret
-    | |-unspecThread(?t, [specAct], ?s, ?m) ?z => eapply unspecCreatedSpec
+    | |-unspecThread(?t, unlocked [], ?s, ?m) ?z => eapply unspecCommit
+    | |-unspecThread(?t, unlocked(?x++[rAct ?a ?b ?c ?d]), ?s, ?m) ?z => eapply unspecRead
+    | |-unspecThread(?t, unlocked(?x++[wAct ?a ?b ?c ?d ?e]), ?s, ?m) ?z => eapply unspecWrite
+    | |-unspecThread(?t, unlocked(?x++[nAct ?a ?b ?c ?d]), ?s, ?m) ?z => eapply unspecCreate
+    | |-unspecThread(?t, unlocked(?x++[fAct ?a ?b ?c ?d]), ?s, ?m) ?z => eapply unspecFork
+    | |-unspecThread(?t, unlocked(?x++[srAct ?a ?b ?c ?d ?e]), ?s, ?m) ?z => eapply unspecSpecret
+    | |-unspecThread(?t, locked ?x, ?s, ?m) ?z => eapply unspecLocked
+    | |-unspecThread(?t, unlocked[rAct ?a ?b ?c ?d], ?s, ?m) ?z => eapply unspecRead
+    | |-unspecThread(?t, unlocked[wAct ?a ?b ?c ?d ?e], ?s, ?m) ?z => eapply unspecWrite
+    | |-unspecThread(?t, unlocked[nAct ?a ?b ?c ?d], ?s, ?m) ?z => eapply unspecCreate
+    | |-unspecThread(?t, unlocked[fAct ?a ?b ?c ?d], ?s, ?m) ?z => eapply unspecFork
+    | |-unspecThread(?t, unlocked[srAct ?a ?b ?c ?d ?e], ?s, ?m) ?z => eapply unspecSpecret
   end. 
 
 (*---------------------------------Theorems---------------------------------------------*)
-
+ 
 Theorem commitPoolUnspecUnchanged : forall T, commitPool T -> T = unspecPoolAux T. 
 Proof.
   intros. apply Extensionality_Ensembles. unfold Same_set. unfold Included. split.  
   {intros. destruct x. destruct p. destruct p. 
    econstructor. econstructor. eassumption. reflexivity. unfold commitPool in H.  
    apply H in H0. subst. eauto. constructor. }
-  {intros. inv H0. inv H1. inv H4. unfold commitPool in H. copy H0. apply H in H0. subst. 
-   inv H2; try invertListNeq. inv H3. auto. }
+  {intros. inv H0. inv H1. inv H4. unfold commitPool in H. copy H0. apply H in H0. subst.
+   inv H2; try invertListNeq. inv H3; auto. }
 Qed. 
 
 Theorem unspecUnionComm : forall T1 T2, unspecPoolAux (tUnion T1 T2) = 
@@ -153,19 +156,19 @@ Proof.
 Qed. 
 
 Theorem raw_unspecHeapRBNew : forall H x S A,
-                            raw_heap_lookup x H = Some(sempty (S::A)) ->
+                            raw_heap_lookup x H = Some(sempty (aCons S A)) ->
                             raw_unspecHeap H = raw_unspecHeap (raw_remove H x). 
 Proof.
   induction H; intros. 
   {inv H. }
   {simpl in *. destruct a. destruct (beq_nat x i) eqn:eq. 
-   {inv H0. auto. }
+   {inv H0. unfold aCons. destruct A; auto. }
    {erewrite IHlist; eauto. destruct i0; simpl; auto. }
   }
 Qed. 
 
 Theorem unspecHeapRBNew : forall H x S A,
-                            heap_lookup x H = Some(sempty (S::A)) ->
+                            heap_lookup x H = Some(sempty (aCons S A)) ->
                             unspecHeap H = unspecHeap (remove H x). 
 Proof.
   intros. destruct H. simpl in *. eapply raw_unspecHeapRBNew in H0. 
@@ -173,26 +176,27 @@ Proof.
 Qed. 
 
 Theorem raw_unspecHeapRBWrite : forall H x sc S A TID N,
-                                  raw_heap_lookup x H = Some(sfull sc (Empty_set tid) (S::A) TID N) ->
+                                  raw_heap_lookup x H = Some(sfull sc (Empty_set tid) (aCons S A) TID N) ->
                                   raw_unspecHeap (raw_replace x (sempty sc) H) = (raw_unspecHeap H). 
 Proof.
   induction H; intros. 
   {inv H. }
   {simpl in *. destruct a. destruct (beq_nat x i) eqn:eq. 
-   {inv H0. destruct sc. simpl. apply beq_nat_true in eq. subst. auto. auto. }
+   {simpl in *. inv H0. destruct (commit sc) eqn:eq2. 
+    unfold commit. destruct A; simpl; auto. apply beq_nat_true in eq. subst; auto. 
+    apply beq_nat_true in eq; subst; auto. auto. }
    {simpl in *. erewrite IHlist; eauto. }
   }
 Qed. 
 
 Theorem unspecHeapRBWrite : forall H x sc S A TID N,
-                              heap_lookup x H = Some(sfull sc (Empty_set tid) (S::A) TID N) ->
+                              heap_lookup x H = Some(sfull sc (Empty_set tid) (aCons S A) TID N) ->
                               unspecHeap (replace x (sempty sc) H) = (unspecHeap H). 
 Proof.
   intros. destruct H. simpl in *. eapply raw_unspecHeapRBWrite in H0. 
   eapply rawHeapsEq. auto. 
 Qed. 
 
-  
 Theorem raw_unspecHeapRBRead : forall H x sc ds S ds' t N,
                    raw_heap_lookup x H = Some (sfull sc ds S t N) ->
                    raw_unspecHeap (raw_replace x (sfull sc ds' S t N) H) = raw_unspecHeap H.
@@ -200,7 +204,7 @@ Proof.
   induction H; intros. 
   {inv H. }
   {simpl in *. destruct a. destruct (beq_nat x i) eqn:eq. 
-   {inv H0. destruct sc; auto. simpl. apply beq_nat_true in eq. subst; auto. }
+   {simpl. inv H0. apply beq_nat_true in eq. subst. destruct (commit sc); auto. }
    {simpl. erewrite IHlist; eauto. }
   }
 Qed. 
@@ -238,63 +242,58 @@ Qed.
 
 Theorem unspecThreadTotal : forall t, exists t', unspecThread t t'. 
 Proof.
-  intros. destruct t. destruct p. destruct p. destructLast a0. 
-  {eauto. }
-  {invertHyp. destruct x; econstructor; unspecThreadTac; eauto. }
+  intros. destruct t. destruct p. destruct p. destruct a. eauto. 
+  destructLast l0. eauto. invertHyp. destruct x; econstructor; unspecThreadTac; auto.  
 Qed. 
+
+Hint Resolve app_nil_l.
 
 Theorem unspecLastAct : forall tid A s2 M M' t,
                          actionTerm A M' ->
-                         (unspecThread (tid, [A], s2, M) t <->
-                          unspecThread (tid, nil, s2, M') t). 
+                         (unspecThread (tid, unlocked[A], s2, M) t <->
+                          unspecThread (tid, unlocked nil, s2, M') t). 
 Proof.
   intros. split; intros. 
-  {inversion H0; subst;    
+  {inversion H0; subst; inv H6; 
    match goal with
        |H:[?A]=?s++[?a], H':actionTerm ?ac ?m |- _ =>
         destruct s; inv H; try invertListNeq; inv H'
    end; auto. }
-  {inversion H0; subst; try invertListNeq.
-   inv H; unspecThreadTac; auto. }
+  {inv H0; try solve[inv H6; invertListNeq]. inv H; unspecThreadTac; rewrite app_nil_l; eauto. 
+  }
 Qed. 
 
 Theorem unspecTwoActs : forall tid A1 As s2 M M' t,
-                         unspecThread (tid, (A1::As), s2, M') t <->
-                         unspecThread (tid, (A1::As), s2, M) t. 
+                         unspecThread (tid, (aCons A1 As), s2, M') t <->
+                         unspecThread (tid, (aCons A1 As), s2, M) t. 
 Proof.
   intros. split; intros. 
-  {inversion H; subst;
-   match goal with
-       |H:?A::?As=?s++[?a] |- _ => rewrite H; eauto
-   end. }
-  {inversion H; subst;
-   match goal with
-       |H:?A::?As=?s++[?a] |- _ => rewrite H; eauto
-   end. }
+  {inv H; destruct As; simpl in *; try inv H2; try invertListNeq; try(inv H5; rewrite H0; eauto).
+   eauto. }
+  {inv H; destruct As; simpl in *; try inv H2; try invertListNeq; try(inv H5; rewrite H0; eauto). 
+   eauto. }
 Qed. 
 
 Theorem unspecTwoActs' : forall tid A1 A2 As s2 M M' t,
-                         unspecThread (tid, (A1::A2::As), s2, M') t <->
-                         unspecThread (tid, (A2 :: As), s2, M) t. 
+                         unspecThread (tid, (aCons A1 (aCons A2 As)), s2, M') t <->
+                         unspecThread (tid, (aCons A2 As), s2, M) t. 
 Proof.
   intros. split; intros. 
-  {inversion H; subst;  
-   match goal with
-     |H:?A1::?A2::?As=?s++[?a] |- _ =>
-      apply listAlign in H; inversion H as [Ex1 Ex2]; rewrite Ex2; eauto
-   end. 
+  {inv H; destruct As; simpl in *; try invertListNeq. 
+   {inv H5. apply listAlign in H0. invertHyp. rewrite H. eauto. }
+   {inv H5. apply listAlign in H0. invertHyp. rewrite H. eauto. }
+   {inv H5. apply listAlign in H0. invertHyp. rewrite H. eauto. }
+   {inv H5. apply listAlign in H0. invertHyp. rewrite H. eauto. }
+   {inv H5. apply listAlign in H0. invertHyp. rewrite H. eauto. }
+   {eauto. }
   }
-  {inversion H; subst; 
-   match goal with
-       |H:?A::?As=?s++[?a] |- _ => rewrite H in *; eauto 
-   end. 
-  }
+  {inv H; destruct As; simpl in *; try invertListNeq; eauto; inv H5; rewrite H0; 
+   rewrite app_comm_cons; eauto. }
 Qed.
 
 Theorem unspecDeterm : forall t t' t'', unspecThread t t' -> unspecThread t t'' -> t' = t''. 
 Proof.
-  intros.
-  inv H; inv H0; auto; try solve[invertListNeq]; 
+  intros. inv H; inv H0; eauto; try solve[invertListNeq]; subst; inv H5;
   match goal with
        |H:?s++[?a]=?s'++[?a'], H':decompose ?M ?E ?e |- _ => 
         apply lastElementEq in H; inv H
@@ -330,89 +329,132 @@ Ltac helper :=
 
 Theorem raw_unspecHeapAddWrite : forall x sc H a b TID N,
                                raw_heap_lookup x H = Some(sempty sc) -> 
-                               raw_unspecHeap (raw_replace x (sfull sc (Empty_set tid) (a::b) TID N) H) = 
+                               raw_unspecHeap (raw_replace x (sfull sc (Empty_set tid) (aCons a b) TID N) H) = 
                                raw_unspecHeap H. 
 Proof.
   induction H; intros. 
   {inv H. }
   {simpl in *. destruct a. destruct (beq_nat x i) eqn:eq. 
-   {inv H0. apply beq_nat_true in eq. subst. destruct sc; auto. }
+   {simpl. inv H0. apply beq_nat_true in eq. subst. destruct (commit sc); auto. 
+    destruct b; simpl; auto. }
    {simpl. erewrite IHlist; eauto. }
   }
 Qed. 
 
 Theorem unspecHeapAddWrite : forall x sc H a b TID N,
                                heap_lookup x H = Some(sempty sc) -> 
-                               unspecHeap (replace x (sfull sc (Empty_set tid) (a::b) TID N) H) = unspecHeap H. 
+                               unspecHeap (replace x (sfull sc (Empty_set tid) (aCons a b) TID N) H) = unspecHeap H. 
 Proof.
   intros. destruct H. simpl in *. eapply raw_unspecHeapAddWrite in H0; eauto.
   apply rawHeapsEq; eauto. 
 Qed. 
 
 Theorem raw_unspecHeapExtend : forall res H a b,
-                                 res = raw_extend(sempty (a::b)) H -> 
+                                 res = raw_extend(sempty (aCons a b)) H -> 
                                  raw_unspecHeap (SND res) = raw_unspecHeap H.
 Proof. 
   induction H; intros. 
-  {simpl in H. inv H. auto. }
-  {simpl in *. destruct a. inv H0. auto. }
+  {simpl in H. inv H. simpl. destruct b; simpl; auto. }
+  {simpl in *. destruct a. inv H0. simpl. destruct b; simpl; auto. }
 Qed.
   
 Theorem unspecHeapExtend : forall x H H' a b,
-                             (x,H')=extend(sempty (a::b)) H -> 
+                             (x,H')=extend(sempty (aCons a b)) H -> 
                              unspecHeap H' = unspecHeap H.
 Proof. 
   intros. destruct H. simpl in *. inv H0. 
   eapply rawHeapsEq. eapply raw_unspecHeapExtend. auto. 
 Qed. 
 
+
+Ltac uCons a b := replace (unlocked (a::b)) with (aCons a (unlocked b)); auto. 
+
 Theorem unspecSpecStep : forall H t H' T t' t'', 
                            spec_step H T t H' T t' -> 
                            unspecPool t t'' -> unspecHeap H = unspecHeap H' /\ unspecPool t' t''. 
 Proof.
   intros. inversion H0; subst.
-  {inv H1; split; auto. helper. erewrite unspecSingleton; eauto. erewrite unspecSingleton.
-   rewrite unspecTwoActs; eauto. eauto. }
-  {inv H1; split; auto. helper. erewrite unspecSingleton; eauto. erewrite unspecSingleton.
-   rewrite unspecTwoActs; eauto. eauto. }
-  {inv H1; split; auto. helper. erewrite unspecSingleton; eauto. erewrite unspecSingleton.
-   rewrite unspecTwoActs; eauto. eauto. }
-  {inv H1; split; auto. helper. erewrite unspecSingleton; eauto. erewrite unspecSingleton.
-   rewrite unspecTwoActs; eauto. eauto. }
-  {inv H1; split; auto. helper. erewrite unspecSingleton; eauto. erewrite unspecSingleton.
-   rewrite unspecTwoActs; eauto. eauto. }
-  {inv H1; split; auto. helper. erewrite unspecSingleton; eauto. erewrite unspecSingleton.
-   rewrite unspecTwoActs; eauto. eauto. }
-  {inv H1; split; auto. helper. erewrite unspecSingleton; eauto. erewrite unspecSingleton.
-   rewrite unspecTwoActs; eauto. eauto. }
-  {inv H1; split; auto. destruct b. 
-   {erewrite unspecSingleton; auto. unfoldTac. rewrite coupleUnion. rewrite unspecUnionComm. 
-    repeat erewrite unspecSingleton; eauto. unfoldTac. rewrite union_empty_r. eauto. 
+  {inv H1; split; auto. helper. inv H3. 
+   {erewrite unspecSingleton; eauto. erewrite unspecSingleton; eauto. }
+   {erewrite unspecSingleton; eauto. erewrite unspecSingleton; eauto. 
+    uCons a b. erewrite unspecTwoActs. eauto. }
+  }
+  {inv H1; split; auto. helper. inv H3. 
+   {erewrite unspecSingleton; eauto. erewrite unspecSingleton; eauto. }
+   {erewrite unspecSingleton; eauto. erewrite unspecSingleton; eauto. 
+    uCons a b. erewrite unspecTwoActs. eauto. }
+  }
+  {inv H1; split; auto. helper. inv H3. 
+   {erewrite unspecSingleton; eauto. erewrite unspecSingleton; eauto. }
+   {erewrite unspecSingleton; eauto. erewrite unspecSingleton; eauto. 
+    uCons a b. erewrite unspecTwoActs. eauto. }
+  }
+  {inv H1; split; auto. helper. inv H3. 
+   {erewrite unspecSingleton; eauto. erewrite unspecSingleton; eauto. }
+   {erewrite unspecSingleton; eauto. erewrite unspecSingleton; eauto. 
+    uCons a b. erewrite unspecTwoActs. eauto. }
+  }
+  {inv H1; split; auto. helper. inv H3. 
+   {erewrite unspecSingleton; eauto. erewrite unspecSingleton; eauto. }
+   {erewrite unspecSingleton; eauto. erewrite unspecSingleton; eauto. 
+    uCons a b. erewrite unspecTwoActs. eauto. }
+  }
+  {inv H1; split; auto. helper. inv H3. 
+   {erewrite unspecSingleton; eauto. erewrite unspecSingleton; eauto. }
+   {erewrite unspecSingleton; eauto. erewrite unspecSingleton; eauto. 
+    uCons a b. erewrite unspecTwoActs. eauto. }
+  }
+  {inv H1; split; auto. helper. inv H3. 
+   {erewrite unspecSingleton; eauto. erewrite unspecSingleton; eauto. }
+   {erewrite unspecSingleton; eauto. erewrite unspecSingleton; eauto. 
+    uCons a b. erewrite unspecTwoActs. eauto. }
+  }
+  {inv H1; split; auto. destruct b.   
+   {simpl. repeat erewrite unspecSingleton; eauto. unfoldTac. rewrite coupleUnion. 
+    rewrite unspecUnionComm. repeat erewrite unspecSingleton; eauto. unfoldTac. rewrite union_empty_l. 
     eauto. }
-   {assert(exists t', unspecThread (tid,a::b,s2,t0) t') by apply unspecThreadTotal. 
+   {destruct l. 
+    {simpl. unfoldTac. rewrite coupleUnion. erewrite unspecSingleton; eauto. rewrite unspecUnionComm. 
+     repeat erewrite unspecSingleton; eauto. unfoldTac. rewrite union_empty_r. eauto. 
+     eapply unspecFork. rewrite app_nil_l. eauto. }
+    {simpl. assert(exists t', unspecThread (tid, aCons a (unlocked l), s2,t0) t') by apply unspecThreadTotal. 
     invertHyp. erewrite unspecSingleton; eauto. unfoldTac. rewrite coupleUnion. 
     rewrite unspecUnionComm. repeat erewrite unspecSingleton; eauto. unfoldTac. rewrite union_empty_r. 
-    eauto. rewrite unspecTwoActs'. eauto. }
+    eauto. rewrite <- unspecTwoActs' in H1. simpl in *. eauto. }
+   }
+  }  
+  {split. symmetry. eapply unspecHeapRBRead; eauto. inv H1. destruct b. 
+   {erewrite unspecSingleton; eauto. erewrite unspecSingleton; eauto. simpl. eauto. }
+   {destruct l. simpl. erewrite unspecSingleton; eauto. erewrite unspecSingleton; eauto.
+    unspecThreadTac; rewrite app_nil_l; eauto. helper. erewrite unspecSingleton; eauto. 
+    erewrite unspecSingleton; eauto. uCons a l. rewrite <- unspecTwoActs'. eauto. }
   }
-  {split. symmetry. eapply unspecHeapRBRead; eauto. inv H1. destruct b. erewrite unspecSingleton; eauto. 
-   erewrite unspecSingleton; eauto. helper. erewrite unspecSingleton; eauto. 
-   erewrite unspecSingleton; eauto. rewrite <- unspecTwoActs'. eauto. }
-  {split. symmetry. eapply unspecHeapAddWrite; eauto. inv H1. destruct b. erewrite unspecSingleton; eauto. 
-   erewrite unspecSingleton; eauto. helper. erewrite unspecSingleton; eauto. 
-   erewrite unspecSingleton; eauto. rewrite <- unspecTwoActs'. eauto. }
-  {split. erewrite <- unspecHeapExtend; eauto. inv H1. destruct b. erewrite unspecSingleton; eauto.
-   erewrite unspecSingleton; eauto. helper. erewrite unspecSingleton; eauto. 
-   erewrite unspecSingleton; eauto. rewrite <- unspecTwoActs'. eauto. }
-  {split; eauto. inv H1. destruct b. 
-   {erewrite unspecSingleton; eauto. unfoldTac. rewrite coupleUnion. rewrite unspecUnionComm. 
-    repeat erewrite unspecSingleton; eauto. unfoldTac. rewrite union_empty_r. eauto. 
-    apply unspecCreatedSpec with(s1':=[specAct]).  auto. eauto. }
-   {assert(exists t', unspecThread(tid,a::b,s2,t0) t') by apply unspecThreadTotal. invertHyp. 
-    erewrite unspecSingleton; eauto. unfoldTac. rewrite coupleUnion. rewrite unspecUnionComm. 
-    repeat erewrite unspecSingleton; eauto. unfoldTac. rewrite union_empty_r. eauto.
-    apply unspecCreatedSpec with (s1':=[specAct]); auto. rewrite unspecTwoActs'; eauto. }
+  {split. symmetry. eapply unspecHeapAddWrite; eauto. inv H1. destruct b. 
+   {erewrite unspecSingleton; eauto. erewrite unspecSingleton; eauto. simpl. eauto. }
+   {destruct l. simpl. erewrite unspecSingleton; eauto. erewrite unspecSingleton; eauto.
+    unspecThreadTac; rewrite app_nil_l; eauto. helper. erewrite unspecSingleton; eauto. 
+    erewrite unspecSingleton; eauto. uCons a l. rewrite <- unspecTwoActs'. eauto.  }
+  }
+  {split. symmetry. eapply unspecHeapExtend; eauto. inv H1. destruct b. 
+   {erewrite unspecSingleton; eauto. erewrite unspecSingleton; eauto. simpl. eauto. }
+   {destruct l. simpl. erewrite unspecSingleton; eauto. erewrite unspecSingleton; eauto.
+    unspecThreadTac; rewrite app_nil_l; eauto. helper. erewrite unspecSingleton; eauto. 
+    erewrite unspecSingleton; eauto. uCons a l. rewrite <- unspecTwoActs'. eauto.  }
+  }
+  {split. symmetry. eauto. inv H1. destruct b. 
+   {unfoldTac. rewrite coupleUnion. erewrite unspecSingleton; eauto. rewrite unspecUnionComm. 
+    erewrite unspecSingleton; eauto. erewrite unspecSingleton; eauto. unfoldTac. 
+    rewrite union_empty_r. eauto. simpl. eauto. }
+   {destruct l. simpl. erewrite unspecSingleton; eauto. unfoldTac. rewrite coupleUnion. 
+    rewrite unspecUnionComm. erewrite unspecSingleton; eauto. erewrite unspecSingleton; eauto. 
+    unfoldTac. rewrite union_empty_r. eauto. unspecThreadTac. rewrite app_nil_l; auto.
+    erewrite unspecSingleton; eauto. assert(exists t', unspecThread(tid,unlocked(a::l), s2, t0) t').
+    apply unspecThreadTotal. invertHyp. unfoldTac. rewrite coupleUnion. rewrite unspecUnionComm. 
+    erewrite unspecSingleton; eauto. erewrite unspecSingleton; eauto. unfoldTac. 
+    rewrite union_empty_r. eauto. uCons a l. rewrite unspecTwoActs'. eauto. }
   }
 Qed. 
+
 
 Theorem unspecSpecMultistep : forall H T H' T' T'', 
                                 spec_multistep H T H' T' -> 
@@ -432,6 +474,9 @@ Ltac rollbackIdemHelper :=
       assert(unspecPoolAux t' = unspecPoolAux t)
     | |- unspecPoolAux(Singleton ?T ?t) = unspecPoolAux(Singleton ?T ?t') =>
       assert(exists t', unspecThread t t') by apply unspecThreadTotal
+    | |- unspecThread ?t ?t'  => assert(exists t'', unspecThread t t'') by
+                                      apply unspecThreadTotal
+    | |- unspecPool ?T ?T' => assert(unspecPoolAux T = T')
   end. 
 
 Theorem rollbackIdempotent : forall tid stack H T H' T' T'', 
@@ -442,34 +487,72 @@ Proof.
   {auto. }
   {inversion H1; subst. apply IHrollback. unfoldTac. rewrite unspecUnionComm in *. 
    destruct s1'. 
-   {unfoldTac. rollbackIdemHelper. repeat erewrite unspecSingleton; eauto. rewrite H. 
+   {unfoldTac. rollbackIdemHelper. repeat erewrite unspecSingleton; simpl; eauto. rewrite H. 
     rewrite <- unspecUnionComm. constructor. }
-   {unfoldTac. rollbackIdemHelper. rollbackIdemHelper. invertHyp. 
-    repeat erewrite unspecSingleton; eauto. rewrite <- unspecTwoActs'. eauto. rewrite H. 
-    rewrite <- unspecUnionComm. constructor. } 
+   {destruct l. 
+    {unfoldTac. simpl; erewrite unspecSingleton; eauto. rewrite <- unspecUnionComm. constructor.
+     erewrite unspecSingleton; eauto. unspecThreadTac. rewrite app_nil_l. auto. }
+    {erewrite unspecSingleton. rewrite <- unspecUnionComm. constructor. simpl.
+     rollbackIdemHelper. invertHyp. erewrite unspecSingleton; eauto. uCons a l; auto.
+     rewrite <- unspecTwoActs'. simpl. eauto. }
+   }
   }
-  {inv H1. apply IHrollback; auto. unfoldTac. rewrite unspecUnionComm. unfoldTac. rollbackIdemHelper. 
-   rewrite coupleUnion. rewrite unspecUnionComm. unfoldTac. rewrite Union_commutative.  
-   erewrite unspecSingleton; eauto. rewrite union_empty_l. destruct s1'. 
-   repeat erewrite unspecSingleton; eauto. rollbackIdemHelper. invertHyp. 
-   repeat erewrite unspecSingleton; eauto. rewrite <- unspecTwoActs'. eauto. rewrite H.  
-   rewrite <- unspecUnionComm. constructor. }
-  {inv H1. apply IHrollback. unfoldTac. rewrite unspecUnionComm. unfoldTac. rollbackIdemHelper. 
-   destruct s1'. repeat erewrite unspecSingleton; eauto. rollbackIdemHelper. invertHyp. 
-   repeat erewrite unspecSingleton; eauto. rewrite <- unspecTwoActs'. eauto. rewrite H. 
-   rewrite <- unspecUnionComm. constructor.  }
-  {inv H1. apply IHrollback. unfoldTac. rewrite unspecUnionComm. unfoldTac. rollbackIdemHelper. 
-   destruct s1'. repeat erewrite unspecSingleton; eauto. rollbackIdemHelper. invertHyp. 
-   repeat erewrite unspecSingleton; eauto. rewrite <- unspecTwoActs'. eauto. rewrite H. 
-   rewrite <- unspecUnionComm. constructor. }
-  {inv H1. apply IHrollback; auto. unfoldTac. repeat rewrite unspecUnionComm. unfoldTac.  
-   replace(unspecPoolAux (Singleton thread (2 :: TID', [specAct; specAct], s2', N))) with tEmptySet.
-   rewrite union_empty_r. rollbackIdemHelper. destruct s1'. repeat erewrite unspecSingleton; eauto. 
-   rollbackIdemHelper. invertHyp. repeat erewrite unspecSingleton; eauto. rewrite <- unspecTwoActs'. 
-   eauto. rewrite H. rewrite <- unspecUnionComm. constructor. erewrite unspecSingleton; eauto. 
-   apply unspecCreatedSpec with (s1':=[specAct]). auto. 
+  {inv H1. apply IHrollback. unfoldTac. rewrite coupleUnion. repeat rewrite unspecUnionComm. 
+   destruct s1'. 
+   {simpl. repeat erewrite unspecSingleton; eauto. unfoldTac. rewrite union_empty_l. 
+    rewrite union_empty_r. rollbackIdemHelper. rewrite unspecUnionComm. 
+    erewrite unspecSingleton; eauto. unfoldTac. rewrite union_empty_r. auto. 
+    rewrite <- H. constructor. }
+   {simpl. destruct l. 
+    {repeat erewrite unspecSingleton; eauto. unfoldTac. rewrite union_empty_r. 
+     rewrite <- unspecUnionComm. constructor. erewrite unspecSingleton; eauto.
+     unspecThreadTac. rewrite app_nil_l. auto. }
+    {repeat erewrite unspecSingleton; eauto. unfoldTac. rewrite union_empty_r. 
+     rewrite <- unspecUnionComm. constructor. rollbackIdemHelper. invertHyp. 
+     erewrite unspecSingleton; eauto. uCons a l; auto. rewrite  <- unspecTwoActs'. simpl. 
+     eauto. }
+   }
+  }
+  {inversion H1; subst. apply IHrollback. unfoldTac. rewrite unspecUnionComm in *. 
+   destruct s1'. 
+   {unfoldTac. rollbackIdemHelper. repeat erewrite unspecSingleton; simpl; eauto. rewrite H. 
+    rewrite <- unspecUnionComm. constructor. }
+   {destruct l. 
+    {unfoldTac. simpl; erewrite unspecSingleton; eauto. rewrite <- unspecUnionComm. constructor.
+     erewrite unspecSingleton; eauto. unspecThreadTac. rewrite app_nil_l. auto. }
+    {erewrite unspecSingleton. rewrite <- unspecUnionComm. constructor. simpl.
+     rollbackIdemHelper. invertHyp. erewrite unspecSingleton; eauto. uCons a l; auto.
+     rewrite <- unspecTwoActs'. simpl. eauto. }
+   }
+  }
+  {inversion H1; subst. apply IHrollback. unfoldTac. rewrite unspecUnionComm in *. 
+   destruct s1'. 
+   {unfoldTac. rollbackIdemHelper. repeat erewrite unspecSingleton; simpl; eauto. rewrite H. 
+    rewrite <- unspecUnionComm. constructor. }
+   {destruct l. 
+    {unfoldTac. simpl; erewrite unspecSingleton; eauto. rewrite <- unspecUnionComm. constructor.
+     erewrite unspecSingleton; eauto. unspecThreadTac. rewrite app_nil_l. auto. }
+    {erewrite unspecSingleton. rewrite <- unspecUnionComm. constructor. simpl.
+     rollbackIdemHelper. invertHyp. erewrite unspecSingleton; eauto. uCons a l; auto.
+     rewrite <- unspecTwoActs'. simpl. eauto. }
+   }
+  }
+  {inv H1. unfoldTac. apply IHrollback. repeat rewrite unspecUnionComm. destruct s1'. 
+   {simpl. repeat erewrite unspecSingleton; eauto. unfoldTac. repeat rewrite union_empty_r.
+    rollbackIdemHelper. rewrite unspecUnionComm. erewrite unspecSingleton; eauto.
+    unfoldTac. rewrite union_empty_r; auto. rewrite <- H. constructor. }
+   {simpl. destruct l. 
+    {repeat erewrite unspecSingleton; eauto. unfoldTac. rewrite union_empty_r. 
+     rewrite <- unspecUnionComm. constructor. erewrite unspecSingleton; eauto.
+     unspecThreadTac. rewrite app_nil_l. auto. }
+    {repeat erewrite unspecSingleton; eauto. unfoldTac. rewrite union_empty_r. 
+     rewrite <- unspecUnionComm. constructor. rollbackIdemHelper. invertHyp. 
+     erewrite unspecSingleton; eauto. uCons a l; auto. rewrite  <- unspecTwoActs'. simpl. 
+     eauto. }
+   }
   }
 Qed. 
+
 
 Theorem specStepChangeUnused : forall H T T' t t' H',
                                  spec_step H T t H' T t' ->
