uniqueHeap/classifiedStep.v
@@ -5,144 +5,153 @@ Require Import Heap.
 Require Import sets. 
 Require Import Coq.Sets.Ensembles. 
 
+Inductive SPEC : actionStack -> Prop :=
+|lockSpec : forall s, SPEC (locked s)
+|unlockedSpec : forall a b, SPEC(unlocked (a::b)). 
+
 Inductive prog_step : sHeap -> pool -> pool -> config -> Prop :=
 |BetaRed : forall E e N tid s2 h T t, 
              decompose t E (AST.app (lambda e) N) ->            
-             prog_step h T (tSingleton(tid,nil,s2,t)) 
-                  (OK h T (tSingleton(tid,nil,s2,fill E (open 0 N e))))
+             prog_step h T (tSingleton(tid,(unlocked nil),s2,t)) 
+                  (OK h T (tSingleton(tid,(unlocked nil),s2,fill E (open 0 N e))))
 |ProjL : forall tid s2 E V1 V2 h T t, 
            decompose t E (fst (pair_ V1 V2)) ->
-           prog_step h T (tSingleton(tid,nil,s2,t)) 
-                (OK h T (tSingleton(tid,nil,s2,fill E V1)))
+           prog_step h T (tSingleton(tid,(unlocked nil),s2,t)) 
+                (OK h T (tSingleton(tid,(unlocked nil),s2,fill E V1)))
 |ProjR : forall tid s2 E V1 V2 h T t, 
            decompose t E (snd (pair_ V1 V2)) -> 
-           prog_step h T (tSingleton(tid,nil,s2,t)) 
-                (OK h T (tSingleton(tid,nil,s2,fill E V2)))
+           prog_step h T (tSingleton(tid,(unlocked nil),s2,t)) 
+                (OK h T (tSingleton(tid,(unlocked nil),s2,fill E V2)))
 |Bind : forall tid h E T N M s2 t, decompose t E (bind (ret M) N) ->
-  prog_step h T (tSingleton (tid, nil, s2, t)) 
-       (OK h T (tSingleton (tid,nil,s2,fill E(AST.app N M))))
+  prog_step h T (tSingleton (tid, (unlocked nil), s2, t)) 
+       (OK h T (tSingleton (tid,(unlocked nil),s2,fill E(AST.app N M))))
 |BindRaise : forall tid h E T N M s2 t, decompose t E (bind (raise M) N)->
-  prog_step h T (tSingleton (tid,nil,s2,t)) 
-       (OK h T (tSingleton (tid,nil,s2,fill E (raise M))))
+  prog_step h T (tSingleton (tid,(unlocked nil),s2,t)) 
+       (OK h T (tSingleton (tid,(unlocked nil),s2,fill E (raise M))))
 |Handle : forall tid h E T N M s2 t, decompose t E (handle (raise M) N) ->
-  prog_step h T (tSingleton (tid,nil,s2,t)) 
-       (OK h T (tSingleton (tid,nil,s2,fill E (AST.app  N M))))
+  prog_step h T (tSingleton (tid,(unlocked nil),s2,t)) 
+       (OK h T (tSingleton (tid,(unlocked nil),s2,fill E (AST.app  N M))))
 |HandleRet : forall tid h E T N M s2 t, decompose t E (handle (ret M) N) ->
-  prog_step h T (tSingleton (tid,nil,s2,t)) 
-       (OK h T (tSingleton (tid,nil,s2,fill E (ret M))))
+  prog_step h T (tSingleton (tid,(unlocked nil),s2,t)) 
+       (OK h T (tSingleton (tid,(unlocked nil),s2,fill E (ret M))))
 |Fork : forall tid h T M s2 E t (d:decompose t E (fork M)), 
-          prog_step h T (tSingleton (tid, nil, s2,t)) 
-        (OK h T(tCouple (tid, nil, fAct t E M d :: s2, fill E(ret unit)) 
-                        (1::tid, nil, [specAct], M)))
+          prog_step h T (tSingleton (tid, (unlocked nil), s2,t)) 
+        (OK h T(tCouple (tid, (unlocked nil), fAct t E M d :: s2, fill E(ret unit)) 
+                        (1::tid, (unlocked nil), [], M)))
 |Get : forall TID h h' T N s2 E x s ds writer t (d:decompose t E (get (fvar x))),
-         heap_lookup x h = Some(sfull nil ds s writer N) -> 
-         h' = replace x (sfull nil (Add tid ds TID) s writer N) h ->
-         prog_step h T (tSingleton (TID, nil, s2, t))
-              (OK h' T (tSingleton (TID, nil, rAct x t E d::s2, fill E(ret N))))
+         heap_lookup x h = Some(sfull (unlocked nil) ds s writer N) -> 
+         h' = replace x (sfull (unlocked nil) (Add tid ds TID) s writer N) h ->
+         prog_step h T (tSingleton (TID, (unlocked nil), s2, t))
+              (OK h' T (tSingleton (TID, (unlocked nil), rAct x t E d::s2, fill E(ret N))))
 |Put : forall E x N h h' s2 TID T t (d:decompose t E (put (fvar x) N)), 
-         decompose t E (put (fvar x) N) -> heap_lookup x h = Some(sempty nil) ->
-         h' = replace x (sfull nil (Empty_set tid) nil TID N) h -> 
-         prog_step h T (tSingleton (TID, nil, s2, t)) (OK h' T
-              (tSingleton (TID, nil, wAct x t E N d::s2, fill E(ret unit))))
+         decompose t E (put (fvar x) N) -> heap_lookup x h = Some(sempty (unlocked nil)) ->
+         h' = replace x (sfull (unlocked nil) (Empty_set tid) (unlocked nil) TID N) h -> 
+         prog_step h T (tSingleton (TID, (unlocked nil), s2, t)) (OK h' T
+              (tSingleton (TID, (unlocked nil), wAct x t E N d::s2, fill E(ret unit))))
 |Overwrite : forall t E x N N' h h' h'' T TR TR' S' A s2 ds TID TID' (d:decompose t E (put (fvar x) N)), 
-               heap_lookup x h = Some (sfull nil ds (S'::A) TID' N') ->
-               rollback TID' (S'::A) h TR h' TR' ->
-               h'' = replace x (sfull nil (Empty_set tid) nil TID N) h' -> 
-               prog_step h T (tAdd TR (TID, nil, s2, fill E(put (fvar x) N))) (OK h'' T
-                    (tAdd TR' (TID, nil, wAct x t E N d::s2, fill E (ret unit))))
+               heap_lookup x h = Some (sfull (unlocked nil) ds (aCons S' A) TID' N') ->
+               rollback TID' (aCons S' A) h TR h' TR' ->
+               h'' = replace x (sfull (unlocked nil) (Empty_set tid) (unlocked nil) TID N) h' -> 
+               prog_step h T (tAdd TR (TID, (unlocked nil), s2, fill E(put (fvar x) N))) (OK h'' T
+                    (tAdd TR' (TID, (unlocked nil), wAct x t E N d::s2, fill E (ret unit))))
 |New : forall E h h' x tid t s2 T (d:decompose t E new),
-         (x, h') = extend (sempty nil) h -> 
-         prog_step h T (tSingleton (tid, nil, s2, fill E new)) 
-              (OK h' T (tSingleton (tid, nil, nAct t E d x::s2, fill E(ret(fvar x)))))
+         (x, h') = extend (sempty (unlocked nil)) h -> 
+         prog_step h T (tSingleton (tid, (unlocked nil), s2, fill E new)) 
+              (OK h' T (tSingleton (tid, (unlocked nil), nAct t E d x::s2, fill E(ret(fvar x)))))
 |Spec : forall E M t N tid s2 T h (d:decompose t E (spec M N)), 
-          prog_step h T (tSingleton (tid, nil, s2, t)) (OK h T
-               (tCouple (tid, nil, srAct t E M N d::s2,t) (tid, nil, [specAct; specAct], N))) 
-|SpecJoin : forall t E M N0 N1 tid T h t1 t2 s1 s1' s2 s2',
-              decompose t E (specRun (ret N1) N0) -> s1 = s1' ++ [specAct] ->
-              t1 = (tid,nil,s2, t) -> t2 = (2::tid,s1,s2',M) ->
+          prog_step h T (tSingleton (tid, (unlocked nil), s2, t)) (OK h T
+               (tCouple (tid, (unlocked nil), srAct t E M N d::s2,t) (tid, (unlocked nil), [], N))) 
+|SpecJoin : forall t E M N0 N1 tid T h t1 t2 s1 s2 s2',
+              decompose t E (specRun (ret N1) N0) ->
+              t1 = (tid,(unlocked nil),s2, t) -> t2 = (2::tid,locked s1,s2',M) ->
               prog_step h T (tCouple t1 t2) 
-                   (OK h T (tSingleton(tid,wrapActs s1' N1, s2, fill E (specJoin (ret N1) M)))) 
-|SpecRB : forall t E' h h' tid T T' E M' N0 s2 s1' s2' t1 t2 TRB, 
+                   (OK h T (tSingleton(tid,unlocked (wrapActs s1 N1), s2, fill E (specJoin (ret N1) M)))) 
+|SpecRB : forall t E' h h' tid T T' E M' N0 s2 s1 s2' t1 t2 TRB, 
             decompose t E' (specRun (raise E) N0)->
-            t1 = (tid,nil,s2,t) -> t2 = (2::tid,s1'++[specAct],s2',M') -> 
+            t1 = (tid,(unlocked nil),s2,t) -> t2 = (2::tid,locked s1,s2',M') -> 
             ~ (exists p, thread_lookup TRB (tid) p) -> 
             thread_lookup TRB (2::tid) t2 -> 
             ~ (exists p', thread_lookup T' (2::tid) p') ->
-            rollback (2::tid) [specAct] h TRB h' T' ->
-            prog_step h T (tAdd TRB t1) (OK h' T (tAdd T' (tid, nil, s2, fill E'(raise E))))
+            rollback (2::tid) (locked nil) h TRB h' T' ->
+            prog_step h T (tAdd TRB t1) (OK h' T (tAdd T' (tid, (unlocked nil), s2, fill E'(raise E))))
 |SpecRaise : forall E' N h tid s2 T E t1 t,
                decompose t E' (specJoin(ret N)(raise E)) ->
-               t1 = (tid, nil, s2, t) -> 
+               t1 = (tid, (unlocked nil), s2, t) -> 
                prog_step h T (tSingleton t1) 
-                    (OK h T (tSingleton (tid, nil, s2, fill E' (raise E))))
+                    (OK h T (tSingleton (tid, (unlocked nil), s2, fill E' (raise E))))
 |PopRead : forall TID t s1 s1' s2 M M' N T h x ds E d h', 
-             s1 = s1' ++ [rAct x M' E d] -> In tid ds TID ->
-             heap_lookup x h = Some (sfull nil ds nil t N) ->
-             h' = replace x (sfull nil (Subtract tid ds TID) nil t N) h ->
-             prog_step h T (tSingleton (TID, s1, s2, M)) (OK h' T (tSingleton (TID, s1', (rAct x M' E d)::s2, M)))
+             s1 = unlocked (s1' ++ [rAct x M' E d]) -> In tid ds TID ->
+             heap_lookup x h = Some (sfull (unlocked nil) ds (unlocked nil) t N) ->
+             h' = replace x (sfull (unlocked nil) (Subtract tid ds TID) (unlocked nil) t N) h ->
+             prog_step h T (tSingleton (TID, s1, s2, M)) 
+                       (OK h' T (tSingleton (TID, unlocked s1', (rAct x M' E d)::s2, M)))
 |PopWrite : forall tid t s1 s1' s2 M M' M'' N T h h' x ds a b E d,
-              s1 = s1' ++ [wAct x M' E M'' d] -> heap_lookup x h = Some(sfull nil ds (a::b) t N) ->
-              h' = replace x (sfull nil ds nil t N) -> 
-              prog_step h T (tSingleton (tid, s1, s2, M)) (OK h T (tSingleton (tid, s1', (wAct x M' E M'' d)::s2, M)))
+              s1 = unlocked(s1' ++ [wAct x M' E M'' d]) -> 
+              heap_lookup x h = Some(sfull (unlocked nil) ds (aCons a b) t N) ->
+              h' = replace x (sfull (unlocked nil) ds (unlocked nil) t N) -> 
+              prog_step h T (tSingleton (tid, s1, s2, M))
+                        (OK h T (tSingleton (tid, unlocked s1', (wAct x M' E M'' d)::s2, M)))
 |PopNewFull : forall h h' s1 s1' s2 i tid M' ds s s' t M N T E d, 
-                s1 = s1' ++ [nAct M' E d i] -> heap_lookup i h = Some(sfull s ds s t N) ->
-                h' = replace i (sfull nil ds s' t N) h -> 
-                prog_step h T (tSingleton (tid, s1, s2, M)) (OK h T (tSingleton (tid, s1', nAct M' E d i::s2, M)))
+                s1 = unlocked(s1' ++ [nAct M' E d i]) ->
+                heap_lookup i h = Some(sfull s ds s t N) ->
+                h' = replace i (sfull (unlocked nil) ds s' t N) h -> 
+                prog_step h T (tSingleton (tid, s1, s2, M)) 
+                          (OK h T (tSingleton (tid, unlocked s1', nAct M' E d i::s2, M)))
 |PopNewEmpty : forall h h' s1 s1' s2 i tid M' s M T E d, 
-                 s1 = s1' ++ [nAct M' E d i] -> heap_lookup i h = Some(sempty s) ->
-                  h' = replace i (sempty nil) h -> 
-                 prog_step h T (tSingleton (tid, s1, s2, M)) (OK h T (tSingleton (tid, s1', nAct M' E d i::s2, M)))
-|PopFork : forall h s1 s1' s1'' s1''' s2 s2' tid M' M N T M'' E d, 
-             s1 = s1' ++ [fAct M' E M'' d] -> s1'' = s1''' ++ [specAct] ->
-             prog_step h T (tCouple (tid, s1, s2, M) (1::tid, s1'', s2', N)) (OK h T 
-                  (tCouple (tid, s1', fAct M' E M'' d::s2, M)
-                           (1::tid, s1''', specAct::s2', N)))
-|PopSpec : forall h s1 s1' s1'' s1''' s2 s2' t tid M' M N T E d, 
-             s1 = s1' ++ [srAct t E M N d] -> s1'' = s1''' ++ [specAct] ->
-             prog_step h T (tCouple (tid, s1, s2, M') (1::tid, s1'', s2', N)) (OK h T 
-                  (tCouple (tid, s1', srAct t E M N d::s2, M')
-                           (1::tid, s1''', specAct::s2', N)))
+                 s1 = unlocked(s1' ++ [nAct M' E d i]) -> heap_lookup i h = Some(sempty s) ->
+                  h' = replace i (sempty (unlocked nil)) h -> 
+                 prog_step h T (tSingleton (tid, s1, s2, M))
+                           (OK h T (tSingleton (tid, unlocked s1', nAct M' E d i::s2, M)))
+|PopFork : forall h s1 s1' s1'' s2 s2' tid M' M N T M'' E d, 
+             s1 = unlocked(s1' ++ [fAct M' E M'' d]) -> 
+             prog_step h T (tCouple (tid, s1, s2, M) (1::tid, locked s1'', s2', N)) (OK h T 
+                  (tCouple (tid, unlocked s1', fAct M' E M'' d::s2, M)
+                           (1::tid, unlocked s1'', s2', N)))
+|PopSpec : forall h s1 s1' s2 t tid M' M N T E d, 
+             s1 = unlocked(s1' ++ [srAct t E M N d]) ->
+             prog_step h T (tSingleton (tid, s1, s2, M')) (OK h T 
+                  (tSingleton (tid, unlocked s1', srAct t E M N d::s2, M')))
 .
 
 Inductive spec_step : sHeap -> pool -> pool -> sHeap -> pool -> pool -> Prop :=
-|SBetaRed : forall E e N tid s2 h T t a b, 
-             decompose t E (AST.app (lambda e) N) ->               
-             spec_step h T (tSingleton(tid,a::b,s2,t)) h T (tSingleton(tid,a::b,s2,fill E (open 0 N e)))
-|SProjL : forall tid s2 E V1 V2 h T t a b, 
-           decompose t E (fst (pair_ V1 V2)) -> 
-           spec_step h T (tSingleton(tid,a::b,s2,t)) h T (tSingleton(tid,a::b,s2,fill E V1))
-|SProjR : forall tid a b s2 E V1 V2 h T t, 
-           decompose t E (snd (pair_ V1 V2)) -> 
-           spec_step h T (tSingleton (tid,a::b,s2,t)) h T (tSingleton(tid,a::b,s2,fill E V2))
-|SBind : forall tid h E T N M a b s2 t, decompose t E (bind (ret M) N) ->
-  spec_step h T (tSingleton (tid, a::b, s2, t)) h T (tSingleton (tid,a::b,s2,fill E(AST.app N M)))
-|SBindRaise : forall tid h E T N M a b s2 t, decompose t E (bind (raise M) N) ->
-  spec_step h T (tSingleton(tid,a::b,s2,t)) h T (tSingleton (tid,a::b,s2,fill E (raise M)))
-|SHandle : forall tid h E T N M a b s2 t, decompose t E (handle (raise M) N) ->
-  spec_step h T (tSingleton(tid,a::b,s2,t)) h T (tSingleton (tid,a::b,s2,fill E (AST.app  N M)))
-|SHandleRet : forall tid h E T N M a b s2 t, decompose t E (handle (ret M) N) ->
-  spec_step h T (tSingleton(tid,a::b,s2,t)) h T (tSingleton (tid,a::b,s2,fill E (ret M)))
+|SBetaRed : forall E e N tid s2 h T t s1, 
+             decompose t E (AST.app (lambda e) N) -> SPEC s1 ->             
+             spec_step h T (tSingleton(tid,s1,s2,t)) h T (tSingleton(tid,s1,s2,fill E (open 0 N e)))
+|SProjL : forall tid s2 E V1 V2 h T t s1, 
+           decompose t E (fst (pair_ V1 V2)) -> SPEC s1 ->   
+           spec_step h T (tSingleton(tid,s1,s2,t)) h T (tSingleton(tid,s1,s2,fill E V1))
+|SProjR : forall tid s1 s2 E V1 V2 h T t, 
+           decompose t E (snd (pair_ V1 V2)) -> SPEC s1 ->   
+           spec_step h T (tSingleton (tid,s1,s2,t)) h T (tSingleton(tid,s1,s2,fill E V2))
+|SBind : forall tid h E T N M s1 s2 t, decompose t E (bind (ret M) N) -> SPEC s1 ->   
+  spec_step h T (tSingleton (tid, s1, s2, t)) h T (tSingleton (tid,s1,s2,fill E(AST.app N M)))
+|SBindRaise : forall tid h E T N M s1 s2 t, decompose t E (bind (raise M) N) -> SPEC s1 ->   
+  spec_step h T (tSingleton(tid,s1,s2,t)) h T (tSingleton (tid,s1,s2,fill E (raise M)))
+|SHandle : forall tid h E T N M s1 s2 t, decompose t E (handle (raise M) N) -> SPEC s1 ->   
+  spec_step h T (tSingleton(tid,s1,s2,t)) h T (tSingleton (tid,s1,s2,fill E (AST.app  N M)))
+|SHandleRet : forall tid h E T N M s1 s2 t, decompose t E (handle (ret M) N) -> SPEC s1 ->   
+  spec_step h T (tSingleton(tid,s1,s2,t)) h T (tSingleton (tid,s1,s2,fill E (ret M)))
 |SFork : forall tid h T M b s2 E t (d:decompose t E (fork M)), 
           spec_step h T (tSingleton(tid, b, s2,t)) h T
-               (tCouple (tid, fAct t E M d::b, s2, fill E(ret unit)) (1::tid, [specAct], nil, M))
+               (tCouple (tid, aCons(fAct t E M d) b, s2, fill E(ret unit)) (1::tid, locked nil, nil, M))
 |SGet : forall TID h h' T N b s2 E x s ds writer sc t (d:decompose t E (get(fvar x))),
          heap_lookup x h = Some(sfull sc ds s writer N) -> 
          h' = replace x (sfull sc (Add tid ds TID) s writer N) h ->
          spec_step h T (tSingleton(TID, b, s2, t)) h' T 
-              (tSingleton (TID, rAct x t E d::b, s2, fill E(ret N)))
+              (tSingleton (TID, aCons (rAct x t E d) b, s2, fill E(ret N)))
 |SPut : forall E x N h sc h' b s2 TID T t (d:decompose t E (put (fvar x) N)), 
          heap_lookup x h = Some(sempty sc) ->
-         h' = replace x (sfull sc (Empty_set tid) (wAct x t E N d::b) TID N) h ->
+         h' = replace x (sfull sc (Empty_set tid) (aCons (wAct x t E N d) b) TID N) h ->
          spec_step h T (tSingleton(TID, b, s2, t)) h' T
-              (tSingleton (TID, wAct x t E N d::b, s2, fill E(ret unit)))
+              (tSingleton (TID, aCons (wAct x t E N d) b, s2, fill E(ret unit)))
 |SNew : forall E h h' x tid t b s2 T (d:decompose t E new),
-         (x, h') = extend (sempty (nAct t E d x::b)) h ->
+         (x, h') = extend (sempty (aCons (nAct t E d x) b)) h ->
          spec_step h T (tSingleton(tid, b, s2, t))h' T
-              (tSingleton (tid, nAct t E d x::b, s2, fill E(ret(fvar x))))
+              (tSingleton (tid, aCons (nAct t E d x) b, s2, fill E(ret(fvar x))))
 |SSpec : forall E M t N tid' tid b s2 T h (d:decompose t E (spec M N)), 
           spec_step h T (tSingleton(tid, b, s2, t)) h T
-               (tCouple (tid, srAct t E M N d::b, s2,fill E(specRun M N))
-                        (tid', [specAct; specAct], nil, N))
+               (tCouple (tid, aCons (srAct t E M N d) b, s2,fill E(specRun M N))
+                        (tid', locked nil, nil, N))
 
 .
 
@@ -163,13 +172,10 @@ Theorem specStepSingleton : forall h t h' T t',
 Proof.
   intros. inv H; eauto. Qed. 
 
-
-
-
 Theorem specStepCommitFullIVar:  forall x H H' ds tid M T t t',
                                    spec_step H T t H' T t' ->
-                                   heap_lookup x H = Some(sfull nil ds nil tid M) ->
-                                  exists ds', heap_lookup x H' = Some(sfull nil ds' nil tid M). 
+                                   heap_lookup x H = Some(sfull (unlocked nil) ds (unlocked nil) tid M) ->
+                                  exists ds', heap_lookup x H' = Some(sfull (unlocked nil) ds' (unlocked nil) tid M). 
 Proof. 
   intros. inv H0; try solve[econstructor; eauto]. 
   {destruct (beq_nat x x0) eqn:eq. 
