uniqueHeap/eraseRollbackIdempotent.v
@@ -7,41 +7,42 @@ Require Import Heap.
 Require Import hetList.    
 Require Import sets. 
 Require Import Coq.Sets.Ensembles. 
-
+Require Import unspec. 
 (*Helper theorems for reasoning about the erasure of heaps being rolled back*)
 Theorem raw_eraseHeapRBNew : forall H x S A,
-                           raw_heap_lookup x H = Some(sempty (S::A)) ->
+                           raw_heap_lookup x H = Some(sempty (aCons S A)) ->
                            raw_eraseHeap H = raw_eraseHeap (raw_remove H x). 
 Proof.
   induction H; intros. 
   {inv H. }
   {simpl in *. destruct a. destruct (beq_nat x i) eqn:eq. 
-   {inv H0; auto. }
+   {inv H0; auto. destruct A; auto. }
    {simpl in *. erewrite IHlist; eauto. }
   }
 Qed. 
 
 Theorem eraseHeapRBNew : forall H x S A,
-                           heap_lookup x H = Some(sempty (S::A)) ->
+                           heap_lookup x H = Some(sempty (aCons S A)) ->
                            eraseHeap H = eraseHeap (remove H x). 
 Proof.
   intros. destruct H; simpl in *. apply rawHeapsEq. eapply raw_eraseHeapRBNew; eauto. 
 Qed. 
 
 Theorem raw_eraseHeapRBWrite : forall H x sc S A TID N,
-                      raw_heap_lookup x H = Some(sfull sc (Empty_set tid) (S::A) TID N) ->
+                      raw_heap_lookup x H = Some(sfull sc (Empty_set tid) (aCons S A) TID N) ->
                       raw_eraseHeap H = raw_eraseHeap (raw_replace x (sempty sc) H). 
 Proof.
   induction H; intros. 
   {inv H. }
   {simpl in *. destruct a. destruct (beq_nat x i) eqn:eq. 
-   {inv H0; auto. apply beq_nat_true in eq. subst. destruct sc; auto. }
+   {inv H0; auto. apply beq_nat_true in eq. subst. destruct (commit sc) eqn:eq2; auto. 
+    destruct A; simpl; auto. rewrite eq2. auto. rewrite eq2; auto. simpl. rewrite eq2. auto. }
    {simpl. erewrite IHlist; eauto. }
   }
 Qed. 
 
 Theorem eraseHeapRBWrite : forall H x sc S A TID N,
-                      heap_lookup x H = Some(sfull sc (Empty_set tid) (S::A) TID N) ->
+                      heap_lookup x H = Some(sfull sc (Empty_set tid) (aCons S A) TID N) ->
                       eraseHeap H = eraseHeap (replace x (sempty sc) H). 
 Proof.
   intros. destruct H; simpl in *. apply rawHeapsEq. eapply raw_eraseHeapRBWrite; eauto. 
@@ -68,37 +69,68 @@ Proof.
   {split; auto. }
   {eapply IHrollback. inversion H6. unfold tAdd. unfold Add. rewrite eraseUnionComm. 
    rollbackIdemHelper. destruct s1'. 
-   {repeat erewrite erasePoolSingleton. reflexivity. eauto. eauto. }
-   {apply eraseExists in H6. inv H6. repeat erewrite erasePoolSingleton. reflexivity. 
-    Focus 2. eauto. rewrite <- eraseTwoActs. eauto. }
-   rewrite H4. rewrite <- eraseUnionComm. constructor. symmetry.
-   erewrite <- eraseHeapDependentRead; eauto. }
-  {assert(exists t', eraseThread (TID', fAct M' E N' d::s1', s2, M) t'). eapply erasePoolEraseThread. 
-   eauto. apply Union_intror. constructor. inv H. eapply IHrollback. inv H5. 
-   unfold tAdd. unfold Add.  unfold tCouple. rewrite couple_swap. rewrite coupleUnion. 
-   repeat rewrite eraseUnionComm. erewrite erasePoolSingleton; eauto. rewrite union_empty_l. 
-   rollbackIdemHelper. repeat erewrite erasePoolSingleton. auto. Focus 2. eauto. 
-   destruct s1'. inversion H2; try invertListNeq. inv H8. destruct s1'; inv H10. auto. 
-   invertListNeq. rewrite <- eraseTwoActs. eauto. rewrite H. rewrite <- eraseUnionComm. 
-   constructor. auto. }
-  {inversion H5; subst. apply eraseExists in H5. inv H5. eapply IHrollback. unfold tAdd. 
-   unfold Add. rewrite eraseUnionComm. rollbackIdemHelper. repeat erewrite erasePoolSingleton; eauto. 
-   destruct s1'. inversion H; try invertListNeq. destruct s1'; inv H8. auto. invertListNeq. 
-   rewrite <- eraseTwoActs. eauto. rewrite H1. rewrite <- eraseUnionComm. constructor. 
-   symmetry. eapply eraseHeapRBWrite; eauto. }
-  {inversion H6; subst. apply eraseExists in H6. inv H6. eapply IHrollback. unfold tAdd. 
-   unfold Add. rewrite eraseUnionComm. rollbackIdemHelper. repeat erewrite erasePoolSingleton; eauto. 
-   destruct s1'. inversion H; try invertListNeq. destruct s1'; inv H9. auto. invertListNeq. 
-   rewrite <- eraseTwoActs. eauto. rewrite H2. rewrite <- eraseUnionComm. constructor. 
-   symmetry. eapply eraseHeapRBNew; eauto. }
-  {assert(exists t', eraseThread (TID', srAct M' E M'' N'' d::s1', s2, M) t'). eapply erasePoolEraseThread. 
-   eauto. constructor. apply Union_intror. constructor. inv H. eapply IHrollback. inv H5. 
-   unfold tAdd. unfold Add. repeat rewrite eraseUnionComm.
-   replace(erasePoolAux (Singleton thread (2 :: TID', [specAct; specAct], s2', N))) with (Empty_set ptrm).
-   Focus 2. erewrite erasePoolSingleton; eauto. eapply tEraseCreatedSpec with(s1':=[specAct]); auto. 
-   rewrite union_empty_r. rollbackIdemHelper. 
-   repeat erewrite erasePoolSingleton; eauto. destruct s1'. 
-   inv H2; try invertListNeq. destruct s1'; inv H8. auto. invertListNeq. rewrite <- eraseTwoActs. 
-   eauto. rewrite H. rewrite <- eraseUnionComm. constructor. auto. }
+   {repeat erewrite erasePoolSingleton. reflexivity. eauto. simpl. eauto. }
+   {destruct l. 
+    {erewrite erasePoolSingleton; eauto. simpl. erewrite erasePoolSingleton; eauto.
+     eraseThreadTac. rewrite app_nil_l. auto. }
+    {apply eraseExists in H6. invertHyp. erewrite erasePoolSingleton; eauto. 
+     erewrite erasePoolSingleton; eauto. uCons a l; auto.
+     rewrite <- eraseTwoActs. eauto. }
+   } rewrite H4. rewrite <- eraseUnionComm. constructor. eapply eraseHeapDependentRead. 
+   eauto.
+  }
+  {eapply IHrollback. inv H5. unfoldTac. rewrite coupleUnion. destruct s1'. 
+   {repeat rewrite eraseUnionComm. erewrite erasePoolSingleton; eauto. 
+    erewrite erasePoolSingleton; eauto. rewrite union_empty_r. rewrite <- eraseUnionComm. 
+    constructor. erewrite erasePoolSingleton; eauto. simpl. auto. }
+   {destruct l. 
+    {repeat rewrite eraseUnionComm. erewrite erasePoolSingleton; eauto. 
+     erewrite erasePoolSingleton; eauto. rewrite union_empty_r. rewrite <- eraseUnionComm. 
+     constructor. erewrite erasePoolSingleton; eauto. simpl. eraseThreadTac. 
+     rewrite app_nil_l. auto. }
+    {repeat rewrite eraseUnionComm. assert(exists t, eraseThread(TID',unlocked(a::l),s2,M') t). 
+     apply eraseThreadTotal. invertHyp. erewrite erasePoolSingleton; eauto.
+     erewrite erasePoolSingleton; eauto. rewrite union_empty_r. rewrite <- eraseUnionComm. 
+     constructor. erewrite erasePoolSingleton; eauto. uCons a l. rewrite eraseTwoActs. 
+     eauto. }
+   } auto. 
+  }
+  {eapply IHrollback. inversion H5. unfold tAdd. unfold Add. rewrite eraseUnionComm. 
+   rollbackIdemHelper. destruct s1'. 
+   {repeat erewrite erasePoolSingleton. reflexivity. eauto. simpl. eauto. }
+   {destruct l. 
+    {erewrite erasePoolSingleton; eauto. simpl. erewrite erasePoolSingleton; eauto.
+     eraseThreadTac. rewrite app_nil_l. auto. }
+    {apply eraseExists in H5. invertHyp. erewrite erasePoolSingleton; eauto. 
+     erewrite erasePoolSingleton; eauto. uCons a l; auto.
+     rewrite <- eraseTwoActs. eauto. }
+   } rewrite H3. rewrite <- eraseUnionComm. constructor. symmetry. eapply eraseHeapRBWrite; eauto. }
+  {eapply IHrollback. inversion H6. unfold tAdd. unfold Add. rewrite eraseUnionComm. 
+   rollbackIdemHelper. destruct s1'. 
+   {repeat erewrite erasePoolSingleton. reflexivity. eauto. simpl. eauto. }
+   {destruct l. 
+    {erewrite erasePoolSingleton; eauto. simpl. erewrite erasePoolSingleton; eauto.
+     eraseThreadTac. rewrite app_nil_l. auto. }
+    {apply eraseExists in H6. invertHyp. erewrite erasePoolSingleton; eauto. 
+     erewrite erasePoolSingleton; eauto. uCons a l; auto.
+     rewrite <- eraseTwoActs. eauto. }
+   } rewrite H4. rewrite <- eraseUnionComm. constructor. symmetry. 
+   eapply eraseHeapRBNew; eauto. 
+  }
+  {eapply IHrollback. inv H5. unfoldTac. destruct s1'. 
+   {repeat rewrite eraseUnionComm. erewrite erasePoolSingleton; eauto. 
+    erewrite erasePoolSingleton; eauto. rewrite union_empty_r. rewrite <- eraseUnionComm. 
+    constructor. erewrite erasePoolSingleton; eauto. simpl. auto. }
+   {destruct l. 
+    {repeat rewrite eraseUnionComm. erewrite erasePoolSingleton; eauto. 
+     erewrite erasePoolSingleton; eauto. rewrite union_empty_r. rewrite <- eraseUnionComm. 
+     constructor. erewrite erasePoolSingleton; eauto. simpl. eraseThreadTac. 
+     rewrite app_nil_l. auto. }
+    {repeat rewrite eraseUnionComm. assert(exists t, eraseThread(TID',unlocked(a::l),s2,M') t). 
+     apply eraseThreadTotal. invertHyp. erewrite erasePoolSingleton; eauto.
+     erewrite erasePoolSingleton; eauto. rewrite union_empty_r. rewrite <- eraseUnionComm. 
+     constructor. erewrite erasePoolSingleton; eauto. uCons a l. rewrite eraseTwoActs. 
+     eauto. }
+   } auto.
+  }
 Qed. 
- 
