uniqueHeap/errorIFF.v
@@ -13,21 +13,21 @@ Require Import classifiedStep.
 Require Import SpecLib.
 
 Theorem raw_eraseFull : forall H x N tid ds,
-                          raw_heap_lookup x H = Some(sfull nil ds nil tid N) ->
+                          raw_heap_lookup x H = Some(sfull (unlocked nil) ds (unlocked nil) tid N) ->
                           raw_heap_lookup x (raw_eraseHeap H) = Some(pfull (eraseTerm N)). 
 Proof.
   induction H; intros. 
   {inv H. }
   {simpl in *. destruct a. destruct (beq_nat x i) eqn:eq. 
    {inv H0. simpl. rewrite eq. auto. }
-   {apply IHlist in H0. destruct i0. destruct a. simpl. rewrite eq. auto. 
-    auto. destruct a. destruct a0. simpl. rewrite eq. auto. simpl. 
+   {apply IHlist in H0. destruct i0. destruct (commit a). simpl. rewrite eq. auto. 
+    auto. destruct (commit a). destruct (commit a0). simpl. rewrite eq. auto. simpl. 
     rewrite eq. auto. auto. }
   }
 Qed. 
 
 Theorem eraseFull : forall H x N tid ds,
-                      heap_lookup x H = Some(sfull nil ds nil tid N) ->
+                      heap_lookup x H = Some(sfull (unlocked nil) ds (unlocked nil) tid N) ->
                       heap_lookup x (eraseHeap H) = Some(pfull (eraseTerm N)). 
 Proof.
   intros. destruct H. simpl in *. eapply raw_eraseFull; eauto. 
@@ -56,26 +56,15 @@ Proof.
   apply decomposeEq in H5. subst. auto. auto. simpl. auto. eauto.  
 Qed.  
 
-Theorem ltLookup : forall T u x H v, raw_heap_lookup x H = Some v ->
-                                       monotonic u T H -> optLT x u = true. 
-Proof.
-  induction H; intros. 
-  {inv H. }
-  {simpl in *. destruct a. destruct (beq_nat x i) eqn:eq. 
-   {inv H0. inversion H1; subst. apply beq_nat_true in eq. subst; auto. }
-   {eapply IHlist; eauto. inversion H1; subst. eapply monotonicLowerUB; eauto. }
-  }
-Qed. 
-
 Theorem raw_eraseFull' : forall H x N u, 
                        monotonic u ivar_state H ->
                        raw_heap_lookup x (raw_eraseHeap H) = Some(pfull (eraseTerm N)) ->
-                       exists tid ds, raw_heap_lookup x H = Some(sfull nil ds nil tid N). 
+                       exists tid ds, raw_heap_lookup x H = Some(sfull (unlocked nil) ds (unlocked nil) tid N). 
 Proof.
   induction H; intros. 
-  {inv H0. }
-  {simpl in H0. destruct a eqn:eq1. destruct i0 eqn:eq2. 
-   {destruct a0. 
+  {inv H0. } 
+  {simpl in *. destruct a eqn:eq1. destruct i0 eqn:eq2. 
+   {destruct (commit a0). 
     {simpl in *. destruct (beq_nat x i). inv H1. eapply IHlist in H1. invertHyp. eauto. 
     inversion H0; subst. eauto. }
     {eapply IHlist in H1. invertHyp. simpl in *. destruct (beq_nat x i) eqn:eq4. 
@@ -85,10 +74,11 @@ Proof.
      {subst. inversion H0; subst. eauto. }
     }
    }
-   {destruct a0. 
-    {destruct a1. 
-     {simpl in *. destruct (beq_nat x i) eqn:eq4. inv H1. apply eraseTermUnique in H3.
-      subst; eauto. eapply IHlist in H1. auto. inversion H0; subst. eauto. }
+   {destruct (commit a0) eqn:eq5. 
+    {destruct (commit a1)eqn:eq6. 
+     {simpl in *. destruct (beq_nat x i) eqn:eq4. inv H1. apply eraseTermUnique in H3. subst.
+      destruct a0; inv eq5. destruct a1; inv eq6. destruct l; inv H2. destruct l0; inv H3.
+      eauto. eapply IHlist in H1; eauto. inv H0. eauto. }
      {simpl in *. destruct (beq_nat x i). inv H1. eapply IHlist in H1. auto. 
       inversion H0; subst. eauto. }
     }
@@ -104,7 +94,7 @@ Qed.
 
 Theorem eraseFull' : forall H x N, 
                        heap_lookup x (eraseHeap H) = Some(pfull (eraseTerm N)) ->
-                       exists tid ds, heap_lookup x H = Some(sfull nil ds nil tid N). 
+                       exists tid ds, heap_lookup x H = Some(sfull (unlocked nil) ds (unlocked nil) tid N). 
 Proof.
   intros. destruct H. simpl in *. eapply raw_eraseFull' in H0; eauto. 
 Qed. 
@@ -122,45 +112,24 @@ Proof.
 Axiom UnionSingletonEq : forall T T' a b, tUnion T (tSingleton a) = tUnion T' (tSingleton b) -> 
                                           tIn T' a -> T = tUnion (Subtract thread T' a) (tSingleton b).
 
-Theorem specStepCommitFullIVar:  forall x H H' ds tid M T t t',
-                                   spec_step H T t H' T t' ->
-                                   heap_lookup x H = Some(sfull nil ds nil tid M) ->
-                                  exists ds', heap_lookup x H' = Some(sfull nil ds' nil tid M). 
-Proof. 
-  intros. inv H0; try solve[econstructor; eauto]. 
-  {destruct (beq_nat x x0) eqn:eq. 
-   {apply beq_nat_true in eq. subst. eapply lookupDeterministic in H2; eauto. inv H2. 
-    exists (Add tid ds0 TID). erewrite HeapLookupReplace; eauto. }
-   {eapply lookupReplaceNeq in H1; eauto. intros c. apply beq_nat_false in eq. contradiction. }
-  }
-  {destruct (beq_nat x x0) eqn:eq. 
-   {apply beq_nat_true in eq. subst. eapply lookupDeterministic in H2; eauto. inv H2. }
-   {eapply lookupReplaceNeq in H1; eauto. apply beq_nat_false in eq. auto. }
-  }
-  {destruct H; simpl in *. destruct h. 
-   {inv H1. }
-   {exists ds. destruct p. simpl in *. destruct (beq_nat x i) eqn:eq. 
-    {inv H1. inversion H2; subst. simpl. inversion m; subst. clear H3. 
-     destruct (beq_nat x (S i)) eqn:eq2. apply beq_nat_true in eq. apply beq_nat_true in eq2. 
-     subst. assert(i <>  S i). omega. contradiction. rewrite eq. auto. }
-    {inversion H2; subst. simpl. inversion m; subst. copy H1. eapply ltLookup in H1; eauto. 
-     simpl in *. destruct (lt_dec x i). Focus 2. inv H1. assert(beq_nat x (S i) = false). 
-     apply beq_nat_false_iff. omega. rewrite H0. rewrite eq. auto. }
-   }
-  }
-Qed.
+Ltac invertActList :=
+  match goal with
+      |H:aCons ?A ?b = locked nil |- _ => destruct b; inv H
+      |H:aCons ?A ?b = unlocked nil |- _ => destruct b; inv H
+  end. 
 
 Theorem spec_multi_false : forall T T' tid s1 x M' E N d s2 M H H' a b c,
-                             spec_multistep H (tUnion T (tSingleton(tid,nil,s2,M'))) H'
-                                            (tUnion T' (tSingleton(tid,s1++[wAct x M' E N d],s2,M))) ->
-                             heap_lookup x H = Some(sfull nil a nil b c) ->
+                             spec_multistep H (tUnion T (tSingleton(tid,unlocked nil,s2,M'))) H'
+                                            (tUnion T' (tSingleton(tid,unlocked(s1++[wAct x M' E N d]),s2,M))) ->
+                             heap_lookup x H = Some(sfull (unlocked nil) a (unlocked nil) b c) ->
                              False. 
 Proof.
   intros. genDeps{a; b; c}. dependent induction H0; intros.
   {subst. unfoldSetEq x. eqIn H. apply H in H2. inversion H2; subst. 
-   {assert(thread_lookup(tAdd T'(tid,s1++[wAct x0 M' E N d],s2,M)) tid (tid,nil,s2,M')). 
+   {assert(thread_lookup(tAdd T'(tid,unlocked(s1++[wAct x0 M' E N d]),s2,M)) tid (tid,unlocked nil,s2,M')). 
     econstructor. econstructor;eauto. eauto. 
-    assert(thread_lookup(tAdd T'(tid,s1++[wAct x0 M' E N d],s2,M)) tid (tid,s1++[wAct x0 M' E N d],s2,M)). 
+    assert(thread_lookup(tAdd T'(tid,unlocked(s1++[wAct x0 M' E N d]),s2,M)) tid 
+                        (tid,unlocked(s1++[wAct x0 M' E N d]),s2,M)). 
     econstructor. apply Union_intror. auto. auto. eapply uniqueThreadPool in H4; eauto.
     inv H4. invertListNeq. }
    {inv H3. invertListNeq. }
@@ -168,7 +137,7 @@ Proof.
   {copy x. copy H. apply specStepSingleton in H. invertHyp. unfoldSetEq x. eqIn H. apply H in H5. 
    inversion H5; subst. eapply specStepCommitFullIVar in H1; eauto. invertHyp.
    {copy H2. eapply UnionSingletonEq in H2; auto. subst. 
-    eapply IHspec_multistep with (T0 := (tUnion (Subtract thread T x1) (tAdd t' (tid,nil,s2,M')))); eauto. 
+    eapply IHspec_multistep with (T0 := (tUnion (Subtract thread T x1) (tAdd t' (tid,unlocked nil,s2,M')))); eauto. 
     apply EqJMeq. eqSets. 
     {inversion H2; subst. inversion H8; subst. constructor. constructor. auto. 
      inv H9. constructor. apply Union_intror. apply Union_intror. auto. constructor. 
@@ -179,46 +148,49 @@ Proof.
    }
    {inv H6. inversion H3;try solve[ unfoldTac; invertHyp; 
     match goal with
-        |H:?a = ?b |- _ => solve[inv H]
-    end]. 
-    {unfoldTac; invertHyp. inv H9. copy d. copy d0. eapply uniqueCtxtDecomp in H6; eauto. 
-     inv H6. inv H9. }
-    {unfoldTac; invertHyp. inv H6. copy d; copy d0. eapply uniqueCtxtDecomp in H6; eauto. 
-     inv H6. inv H10. }
+        |H:?a = ?b |- _ => solve[inv H; invertActList]
+    end];
+    try solve[unfoldTac; invertHyp; 
+     match goal with 
+         |H:(_,_,_,_) = (_,_,_,_) |- _ => inv H
+     end; copy d; copy d0; 
+     match goal with
+         |H:decompose ?M ?E ?e, H' : decompose ?M' ?E' ?e' |- _ => eapply uniqueCtxtDecomp in H; eauto
+     end; invertHyp; cleanup].
     {unfoldTac; invertHyp. inv H6. copy d; copy d0. eapply uniqueCtxtDecomp in H6; eauto. 
      inv H6. inv H10. eapply lookupDeterministic in H1; eauto. inv H1. }
     {unfoldTac; invertHyp. inv H6. copy d; copy d0. eapply uniqueCtxtDecomp in H6; eauto. 
-     inv H6. inv H10. }
-    {unfoldTac; invertHyp. inv H9. copy d; copy d0. eapply uniqueCtxtDecomp in H6; eauto. 
-     inv H6. inv H9. }
+     inv H6. cleanup. clear H11. cleanup. inv H10. }
    }
   }
 Qed. 
 
 Theorem raw_unspecHeapLookupFull : forall H  x a b c,
-                                 raw_heap_lookup x H = Some(sfull nil a nil b c) ->
-                                 raw_heap_lookup x (raw_unspecHeap H) = Some(sfull nil (Empty_set tid) nil b c).
+                                 raw_heap_lookup x H = Some(sfull (unlocked nil) a (unlocked nil) b c) ->
+                                 raw_heap_lookup x (raw_unspecHeap H) = 
+                                 Some(sfull (unlocked nil) (Empty_set tid) (unlocked nil) b c).
 Proof.
   induction H; intros. 
   {inv H. }
   {simpl in *. destruct a. destruct (beq_nat x i) eqn:eq. 
    {inv H0. simpl. rewrite eq. auto. }
-   {apply IHlist in H0. destruct i0. destruct a. simpl; rewrite H0. rewrite eq. 
-    auto. auto. destruct a. destruct a1. simpl. rewrite eq; auto. simpl. rewrite eq; auto. 
+   {apply IHlist in H0. destruct i0. destruct (commit a). simpl; rewrite H0. rewrite eq. 
+    auto. auto. destruct (commit a). destruct (commit a1). simpl. rewrite eq; auto. simpl. rewrite eq; auto. 
     auto. }
   }
 Qed. 
 
 Theorem unspecHeapLookupFull : forall H x a b c,
-                                 heap_lookup x H = Some(sfull nil a nil b c) ->
-                                 heap_lookup x (unspecHeap H) = Some(sfull nil (Empty_set tid) nil b c).
+                                 heap_lookup x H = Some(sfull (unlocked nil) a (unlocked nil) b c) ->
+                                 heap_lookup x (unspecHeap H) = 
+                                 Some(sfull (unlocked nil) (Empty_set tid) (unlocked nil) b c).
 Proof.
   intros. destruct H; simpl in *. eapply raw_unspecHeapLookupFull; eauto. 
 Qed. 
 
 Theorem wfDoubleWrite : forall H T tid s1' x M' E N d s2 M a b c,
-                          wellFormed H (tAdd T (tid,s1'++[wAct x M' E N d],s2,M)) ->
-                          heap_lookup x H = Some(sfull nil a nil b c) -> False. 
+                          wellFormed H (tAdd T (tid,unlocked(s1'++[wAct x M' E N d]),s2,M)) ->
+                          heap_lookup x H = Some(sfull (unlocked nil) a (unlocked nil) b c) -> False. 
 Proof.
   intros. inv H0. inv H3. unfoldTac. rewrite unspecUnionComm in H4. erewrite unspecSingleton in H4.
   Focus 2. eapply unspecWrite. auto. eapply unspecHeapLookupFull in H1; eauto. 
@@ -250,5 +222,10 @@ Proof.
   {apply SingletonEq in H6. subst. copy d. apply decomposeEq in H6. subst. 
    rewrite eraseFill in H4. copy d. rewrite <- decomposeErase in H6; eauto. 
    rewrite eraseFill in H6. simpl in *. eapply pctxtUnique in H4; eauto. inv H4. inv H8. }
-  {symmetry in H6. apply SingletonNeqEmpty in H6. inversion H6. }
+  {symmetry in H8. apply SingletonNeqEmpty in H8. contradiction. }
 Qed. 
+
+
+
+
+
